PREFIX altr-ext: <http://www.w3.org/ns/dx/conneg/altr-ext#>
PREFIX dcat: <http://www.w3.org/ns/dcat#>
PREFIX dcterms: <http://purl.org/dc/terms/>
PREFIX geo: <http://www.opengis.net/ont/geosparql#>
PREFIX owl: <http://www.w3.org/2002/07/owl#>
PREFIX prez: <https://prez.dev/>
PREFIX prof: <http://www.w3.org/ns/dx/prof/>
PREFIX rdf: <http://www.w3.org/1999/02/22-rdf-syntax-ns#>
PREFIX rdfs: <http://www.w3.org/2000/01/rdf-schema#>
PREFIX sh: <http://www.w3.org/ns/shacl#>
PREFIX skos: <http://www.w3.org/2004/02/skos/core#>
PREFIX reg: <http://purl.org/linked-data/registry#>
PREFIX xsd: <http://www.w3.org/2001/XMLSchema#>
PREFIX prov: <http://www.w3.org/ns/prov#>


prez:VocPrezProfile
    a prof:Profile ;
    prez:supportedSearchMethod prez:exactMatch , prez:skosPrefLabel , prez:skosWeighted ;
    dcterms:identifier "vocprez"^^xsd:token ;
    dcterms:description "A system profile for VocPrez" ;
    skos:prefLabel "VocPrez profile" ;
    altr-ext:constrainsClass prez:VocPrez ;
    altr-ext:hasDefaultResourceFormat "text/anot+turtle" ;
    altr-ext:hasNodeShape [
        a sh:NodeShape ;
        sh:targetClass prez:SchemesList ;
        altr-ext:hasDefaultProfile <https://w3id.org/profile/vocpub>
    ] , [
        a sh:NodeShape ;
        sh:targetClass prez:VocPrezCollectionList ;
        altr-ext:hasDefaultProfile <https://w3id.org/profile/vocpub>
    ] , [
        a sh:NodeShape ;
        sh:targetClass skos:Collection ;
        altr-ext:hasDefaultProfile <https://w3id.org/profile/vocpub>
    ] , [
        a sh:NodeShape ;
        sh:targetClass skos:Concept ;
        altr-ext:hasDefaultProfile <https://w3id.org/profile/vocpub>
    ] , [
        a sh:NodeShape ;
        sh:targetClass skos:ConceptScheme ;
        altr-ext:hasDefaultProfile <https://w3id.org/profile/vocpub>
    ]
    .

<https://www.w3.org/TR/vocab-dcat/>
    a prof:Profile , prez:VocPrezProfile ;
    dcterms:description "Dataset Catalog Vocabulary (DCAT) is a W3C-authored RDF vocabulary designed to facilitate interoperability between data catalogs" ;
    dcterms:identifier "dcat"^^xsd:token ;
    dcterms:title "DCAT" ;
    altr-ext:constrainsClass
        dcat:Catalog ,
        dcat:Dataset ,
        prez:VocPrezHome ;
    altr-ext:hasDefaultResourceFormat "text/anot+turtle" ;
    altr-ext:hasResourceFormat
        "application/ld+json" ,
        "application/rdf+xml" ,
        "text/anot+turtle" ,
        "text/turtle" ;
.

<https://w3id.org/profile/vocpub>
    a prof:Profile , prez:VocPrezProfile ;
    dcterms:description "This is a profile of the taxonomy data model SKOS - i.e. SKOS with additional constraints." ;
    dcterms:identifier "vocpub"^^xsd:token ;
    dcterms:title "VocPub" ;
    altr-ext:hasLabelPredicate skos:prefLabel ;
    altr-ext:constrainsClass
        skos:ConceptScheme ,
        skos:Concept ,
        skos:Collection ,
        prez:SchemesList ,
        prez:VocPrezCollectionList ;
    altr-ext:hasDefaultResourceFormat "text/anot+turtle" ;
    altr-ext:hasResourceFormat
        "application/ld+json" ,
        "application/rdf+xml" ,
        "text/anot+turtle" ,
        "text/turtle" ;
    altr-ext:hasNodeShape [
        a sh:NodeShape ;
        sh:targetClass skos:ConceptScheme ;
        altr-ext:outboundChildren skos:hasTopConcept ;
    ] ;
    altr-ext:hasNodeShape [
        a sh:NodeShape ;
        sh:targetClass skos:Collection ;
        altr-ext:outboundChildren skos:member ;
    ] ;
    altr-ext:hasNodeShape [
        a sh:NodeShape ;
        sh:targetClass skos:ConceptScheme ;
        altr-ext:inboundChildren skos:inScheme ;
    ] ;
    altr-ext:hasNodeShape [
        a sh:NodeShape ;
        sh:targetClass skos:ConceptScheme ;
        altr-ext:relativeProperties skos:broader , skos:narrower ;
    ] ;
    altr-ext:hasNodeShape [
        a sh:NodeShape ;
        sh:targetClass skos:Concept ;
        altr-ext:outboundParents skos:inScheme ;
    ] ;
    altr-ext:hasNodeShape [
        a sh:NodeShape ;
        sh:targetClass prez:SchemesList ;
        sh:path dcterms:publisher, reg:status ;
        sh:sequencePath (
            prov:qualifiedDerivation
            prov:hadRole
        ) ;
    ] ;
    altr-ext:hasNodeShape [
        a sh:NodeShape ;
        sh:targetClass prez:VocPrezCollectionList ;
        sh:path skos:definition ;
    ] ;
.

<https://schema.org>
    a prof:Profile ;
    dcterms:description "Schema.org is a collaborative, community activity with a mission to create, maintain, and promote schemas for structured data on the Internet, on web pages, in email messages, and beyond. " ;
    dcterms:identifier "sdo"^^xsd:token ;
    dcterms:title "schema.org" ;
    altr-ext:constrainsClass
        skos:Dataset ,
        skos:ConceptScheme ,
        skos:Collection ;
    altr-ext:hasDefaultResourceFormat "text/turtle" ;
    altr-ext:hasResourceFormat
        "application/ld+json" ,
        "application/rdf+xml" ,
        "text/anot+turtle" ,
        "text/turtle" ;
.

<https://w3id.org/profile/dd>
    a prof:Profile ;
    dcterms:description "A simple data model to provide items for form drop-down lists. The basic information is an ID & name tuple and the optional extra value is an item's parent. For vocabularies, this is then URI, prefLabel or URI, prefLabel & broader Concept" ;
    dcterms:identifier "dd"^^xsd:token ;
    dcterms:title "Drop-Down List" ;
    altr-ext:constrainsClass
        prez:SchemesList ,
        prez:VocPrezCollectionList ,
        skos:ConceptScheme ,
        skos:Collection ;
    altr-ext:hasDefaultResourceFormat "application/json" ;
    altr-ext:hasResourceFormat
        "application/json" ,
        "text/csv"
.
